Build/Reg.dfy
@@ -1,0 +1,75 @@
+module Build.RegBuilder {
+
+  import opened MapFunction
+  import opened Circ
+  import opened Entity
+  import opened CombineManyParallel
+  import opened SeqBuilder
+  import opened ConservedSubcircuit
+
+  function RegSF(n: nat, si: SI): (so: SO)
+    requires |si.inputs| == n
+    requires |si.state| == n
+  {
+    SO(si.state, si.inputs)
+  }
+
+  lemma RegSFIsManyParallelSeqSF(n: nat, si: SI)
+    requires |si.inputs| == n
+    requires |si.state| == n
+    ensures
+      RegSF(n, si) == ManyParallelSF(SeqRF(), n, si)
+  {
+  }
+
+  function InsertRegMF(old_mf: MapFunction, n: nat): (mf: MapFunction)
+    requires |old_mf.inputs| == n
+    requires |old_mf.state| == n
+    requires |old_mf.outputs| == n
+    requires old_mf.Valid()
+    requires MFIsParallelCopies(old_mf, SeqRF(), n)
+    ensures mf.Valid()
+    ensures MapFunctionsEquiv(old_mf, mf)
+  {
+    var mf := MapFunction(
+      old_mf.inputs, old_mf.outputs, old_mf.state,
+      (si: SI) requires SIValid(si, old_mf.inputs, old_mf.state) =>
+      RegSF(n, si));
+    assert mf.Valid() by {
+      reveal MapFunction.Valid();
+      reveal EntityInserter.Valid();
+      reveal MFIsParallelCopies();
+    }
+    assert MapFunctionsSFEquiv(old_mf, mf) by {
+      reveal EntityInserter.Valid();
+      reveal MapFunction.Valid();
+      forall si: SI | SIValid(si, old_mf.inputs, old_mf.state)
+        ensures old_mf.sf(si) == mf.sf(si)
+      {
+        reveal MFIsParallelCopies();
+        reveal EntityInserter.Valid();
+        RegSFIsManyParallelSeqSF(n, si);
+      }
+      reveal MapFunctionsSFEquiv();
+    }
+    MapFunctionsEquivSFEquiv(old_mf, mf);
+    mf
+  }
+
+  function InsertReg(c: Circuit, n: nat): (r: (Circuit, Entity))
+    requires CircuitValid(c)
+    ensures SimpleInsertion(c, r.0, r.1)
+  {
+    var inserter := SeqInserter();
+    var (new_c, e) := InsertInParallel(c, inserter, n);
+    assert |e.mf.inputs| == n && |e.mf.state| == n && |e.mf.outputs| == n by {
+      reveal EntityInserter.Valid();
+      reveal MFIsParallelCopies();
+    }
+    var mf := InsertRegMF(e.mf, n);
+    var new_e := EntitySwapMF(new_c, e, mf);
+    StillSimpleInsertionAfterEntitySwapMF(c, new_c, e, mf);
+    (new_c, new_e)
+  }
+
+}
