CombineManyParallel.dfy
@@ -1,0 +1,400 @@
+module CombineManyParallel {
+
+  import opened Std.Wrappers
+  import Std.Collections.Seq
+
+  import opened MapFunction
+  import opened MapConnection
+  import opened Utils
+  import opened Circ
+  import opened Entity
+  import opened Subcircuit
+  import opened Connection
+  import opened IslandBundle
+  import opened ConservedSubcircuit
+  import opened CombineParallel
+
+  ghost predicate CombineManyParallelEntitiesRequirements(ib: IslandBundle, rf: RFunction) {
+    && IslandBundleValid(ib)
+    && rf.Valid()
+    && (forall e :: e in ib.es ==> e.Some?)
+    && (forall e :: e in ib.es ==> rf.MFConsistent(e.value.mf))
+  }
+
+  function ManyParallelSF(rf: RFunction, n: nat, si: SI): (so: SO)
+    requires |si.inputs| == rf.input_width * n
+    requires |si.state| == rf.state_width * n
+    requires rf.Valid()
+    decreases n
+  {
+    if n == 0 then
+      SO([], [])
+    else
+      var nm1_si := SI(si.inputs[..(n-1)*rf.input_width], si.state[..(n-1)*rf.state_width]);
+      var n_si := SI(si.inputs[(n-1)*rf.input_width..], si.state[(n-1)*rf.state_width..]);
+      var nm1_so := ManyParallelSF(rf, n-1, nm1_si);
+      reveal RFunction.Valid();
+      var n_so := rf.sf(n_si);
+      SO(nm1_so.outputs + n_so.outputs, nm1_so.state + n_so.state)
+  }
+
+  //function ChunkedInputs(ib: IslandBundle): (r: seq<seq<NP>>)
+  //  requires IslandBundleValid(ib)
+  //  requires (forall e :: e in ib.es ==> e.Some?)
+  //  ensures NoDuplicatesNoIntersections(r)
+  //{
+  //  var chunked_inputs := seq(|ib.es|, (index: nat) requires index < |ib.es| => ib.es[index].value.mf.inputs);
+  //  assert NoDuplicatesNoIntersections(chunked_inputs) by {
+  //    forall index: nat | index < |ib.es|
+  //      ensures Seq.HasNoDuplicates(ib.es[index].value.mf.inputs)
+  //    {
+  //      reveal MapFunction.Valid();
+  //      reveal IslandBundleValid();
+  //      var mf := ib.es[index].value.mf;
+  //    }
+  //    forall index1: nat, index2: nat | index1 < |ib.es| && index2 < |ib.es| && index1 != index2
+  //      ensures SeqsNoIntersection(ib.es[index1].value.mf.inputs, ib.es[index2].value.mf.inputs)
+  //    {
+  //      reveal IslandBundleValid();
+  //      var e1 := ib.es[index1].value;
+  //      var e2 := ib.es[index2].value;
+  //      assert e1.sc !! e2.sc;
+  //      FInputsInSc(ib.c, e1);
+  //      FInputsInSc(ib.c, e2);
+  //      ScNoIntersectionNPsNoIntersection(e1.sc, e2.sc, Seq.ToSet(e1.mf.inputs), Seq.ToSet(e2.mf.inputs));
+  //    }
+  //  }
+  //  chunked_inputs
+  //}
+
+  //function ChunkedOutputs(ib: IslandBundle): (r: seq<seq<NP>>)
+  //  requires IslandBundleValid(ib)
+  //  requires (forall e :: e in ib.es ==> e.Some?)
+  //  ensures NoDuplicatesNoIntersections(r)
+  //{
+  //  var chunked_outputs := seq(|ib.es|, (index: nat) requires index < |ib.es| => ib.es[index].value.mf.outputs);
+  //  assert NoDuplicatesNoIntersections(chunked_outputs) by {
+  //    forall index: nat | index < |ib.es|
+  //      ensures Seq.HasNoDuplicates(ib.es[index].value.mf.outputs)
+  //    {
+  //      reveal MapFunction.Valid();
+  //      reveal IslandBundleValid();
+  //      var mf := ib.es[index].value.mf;
+  //    }
+  //    forall index1: nat, index2: nat | index1 < |ib.es| && index2 < |ib.es| && index1 != index2
+  //      ensures SeqsNoIntersection(ib.es[index1].value.mf.outputs, ib.es[index2].value.mf.outputs)
+  //    {
+  //      reveal IslandBundleValid();
+  //      var e1 := ib.es[index1].value;
+  //      var e2 := ib.es[index2].value;
+  //      assert e1.sc !! e2.sc;
+  //      FOutputsInSc(ib.c, e1);
+  //      FOutputsInSc(ib.c, e2);
+  //      ScNoIntersectionNPsNoIntersection(e1.sc, e2.sc, Seq.ToSet(e1.mf.outputs), Seq.ToSet(e2.mf.outputs));
+  //    }
+  //  }
+  //  chunked_outputs
+  //}
+
+  //function ChunkedState(ib: IslandBundle): (r: seq<seq<CNode>>)
+  //  requires IslandBundleValid(ib)
+  //  requires (forall e :: e in ib.es ==> e.Some?)
+  //  ensures NoDuplicatesNoIntersections(r)
+  //{
+  //  var chunked_state := seq(|ib.es|, (index: nat) requires index < |ib.es| => ib.es[index].value.mf.state);
+  //  assert NoDuplicatesNoIntersections(chunked_state) by {
+  //    forall index: nat | index < |ib.es|
+  //      ensures Seq.HasNoDuplicates(ib.es[index].value.mf.state)
+  //    {
+  //      reveal MapFunction.Valid();
+  //      reveal IslandBundleValid();
+  //    }
+  //    forall index1: nat, index2: nat | index1 < |ib.es| && index2 < |ib.es| && index1 != index2
+  //      ensures SeqsNoIntersection(ib.es[index1].value.mf.state, ib.es[index2].value.mf.state)
+  //    {
+  //      reveal IslandBundleValid();
+  //      var e1 := ib.es[index1].value;
+  //      var e2 := ib.es[index2].value;
+  //      assert e1.sc !! e2.sc;
+  //      StateInSc(ib.c, e1);
+  //      StateInSc(ib.c, e2);
+  //    }
+  //  }
+  //  chunked_state
+  //}
+
+  //function ChunkedStateONPs(ib: IslandBundle): (r: seq<seq<NP>>)
+  //  requires IslandBundleValid(ib)
+  //  requires (forall e :: e in ib.es ==> e.Some?)
+  //  ensures NoDuplicatesNoIntersections(r)
+  //{
+  //  var chunked_state_onps := seq(|ib.es|, (index: nat) requires index < |ib.es| => StateONPsSeq(ib.es[index].value.mf.state));
+  //  assert NoDuplicatesNoIntersections(chunked_state_onps) by {
+  //    forall index: nat | index < |ib.es|
+  //      ensures Seq.HasNoDuplicates(StateONPsSeq(ib.es[index].value.mf.state))
+  //    {
+  //      reveal MapFunction.Valid();
+  //      reveal IslandBundleValid();
+  //      StateONPsSeqNoDuplicates(ib.es[index].value.mf.state);
+  //    }
+  //    forall index1: nat, index2: nat | index1 < |ib.es| && index2 < |ib.es| && index1 != index2
+  //      ensures SeqsNoIntersection(StateONPsSeq(ib.es[index1].value.mf.state), StateONPsSeq(ib.es[index2].value.mf.state))
+  //    {
+  //      reveal IslandBundleValid();
+  //      var e1 := ib.es[index1].value;
+  //      var e2 := ib.es[index2].value;
+  //      StateInSc(ib.c, e1);
+  //      StateInSc(ib.c, e2);
+  //      SeqsNoIntersectionEquiv(e1.mf.state, e2.mf.state);
+  //      SeqsNoIntersectionEquiv(StateONPsSeq(e1.mf.state), StateONPsSeq(e2.mf.state));
+  //    }
+  //  }
+  //  chunked_state_onps
+  //}
+
+  //function ChunkedStateINPs(ib: IslandBundle): (r: seq<seq<NP>>)
+  //  requires IslandBundleValid(ib)
+  //  requires (forall e :: e in ib.es ==> e.Some?)
+  //  ensures NoDuplicatesNoIntersections(r)
+  //{
+  //  var chunked_state_inps := seq(|ib.es|, (index: nat) requires index < |ib.es| => StateINPsSeq(ib.es[index].value.mf.state));
+  //  assert NoDuplicatesNoIntersections(chunked_state_inps) by {
+  //    forall index: nat | index < |ib.es|
+  //      ensures Seq.HasNoDuplicates(StateINPsSeq(ib.es[index].value.mf.state))
+  //    {
+  //      reveal MapFunction.Valid();
+  //      reveal IslandBundleValid();
+  //      StateINPsSeqNoDuplicates(ib.es[index].value.mf.state);
+  //    }
+  //    forall index1: nat, index2: nat | index1 < |ib.es| && index2 < |ib.es| && index1 != index2
+  //      ensures SeqsNoIntersection(StateINPsSeq(ib.es[index1].value.mf.state), StateINPsSeq(ib.es[index2].value.mf.state))
+  //    {
+  //      reveal IslandBundleValid();
+  //      var e1 := ib.es[index1].value;
+  //      var e2 := ib.es[index2].value;
+  //      StateInSc(ib.c, e1);
+  //      StateInSc(ib.c, e2);
+  //      SeqsNoIntersectionEquiv(e1.mf.state, e2.mf.state);
+  //      SeqsNoIntersectionEquiv(StateINPsSeq(e1.mf.state), StateINPsSeq(e2.mf.state));
+  //    }
+  //  }
+  //  chunked_state_inps
+  //}
+
+  //lemma ChunkedNoIntersections(ib: IslandBundle)
+  //  requires IslandBundleValid(ib)
+  //  requires (forall e :: e in ib.es ==> e.Some?)
+  //  ensures
+  //    var chunked_inputs := ChunkedInputs(ib);
+  //    var chunked_outputs := ChunkedOutputs(ib);
+  //    var chunked_state_inps := ChunkedStateINPs(ib);
+  //    var chunked_state_onps := ChunkedStateONPs(ib);
+  //    forall index1: nat, index2: nat :: index1 < |ib.es| && index2 < |ib.es| ==> (
+  //      && SeqsNoIntersection(chunked_inputs[index1], chunked_outputs[index2])
+  //      && SeqsNoIntersection(chunked_state_onps[index1], chunked_inputs[index2])
+  //      && SeqsNoIntersection(chunked_state_inps[index1], chunked_outputs[index2])
+  //    )
+  //  {
+  //    var chunked_inputs := ChunkedInputs(ib);
+  //    var chunked_outputs := ChunkedOutputs(ib);
+  //    var chunked_state_inps := ChunkedStateINPs(ib);
+  //    var chunked_state_onps := ChunkedStateONPs(ib);
+  //    forall index1: nat, index2: nat | index1 < |ib.es| && index2 < |ib.es|
+  //      ensures SeqsNoIntersection(chunked_inputs[index1], chunked_outputs[index2])
+  //      ensures SeqsNoIntersection(chunked_state_onps[index1], chunked_inputs[index2])
+  //      ensures SeqsNoIntersection(chunked_state_inps[index1], chunked_outputs[index2])
+  //    {
+  //      var e1 := ib.es[index1].value;
+  //      var e2 := ib.es[index2].value;
+  //      if (index1 == index2) {
+  //        reveal IslandBundleValid();
+  //        reveal MapFunction.Valid();
+  //      } else {
+  //        reveal IslandBundleValid();
+  //        FAllInSc(ib.c, e1);
+  //        FAllInSc(ib.c, e2);
+  //        reveal NPsInSc();
+  //        reveal MapFunction.Valid();
+  //        StateONPsSeqSame(e1.mf.state);
+  //        StateINPsSeqSame(e1.mf.state);
+  //        ScNoIntersectionNPsNoIntersection(e1.sc, e2.sc, Seq.ToSet(chunked_inputs[index1]), Seq.ToSet(chunked_outputs[index2]));
+  //        ScNoIntersectionNPsNoIntersection(e2.sc, e1.sc, Seq.ToSet(chunked_inputs[index2]), Seq.ToSet(chunked_state_onps[index1]));
+  //        ScNoIntersectionNPsNoIntersection(e2.sc, e1.sc, Seq.ToSet(chunked_outputs[index2]), Seq.ToSet(chunked_state_inps[index1]));
+  //      }
+  //    }
+  //  }
+
+  //lemma UnchunkedStateINPsONPsEquiv(ib: IslandBundle, rf: RFunction)
+  //  requires CombineManyParallelEntitiesRequirements(ib, rf)
+  //  ensures
+  //    var chunked_state := ChunkedState(ib);
+  //    var state := UnchunkSeq(chunked_state, |ib.es|, rf.state_width);
+  //    var chunked_state_inps := ChunkedStateINPs(ib);
+  //    var chunked_state_onps := ChunkedStateONPs(ib);
+  //    && (StateINPsSeq(state) == UnchunkSeq(chunked_state_inps, |ib.es|, rf.state_width))
+  //    && (StateONPsSeq(state) == UnchunkSeq(chunked_state_onps, |ib.es|, rf.state_width))
+  //{
+  //}
+
+  opaque ghost predicate MFIsParallelCopies(mf: MapFunction, rf: RFunction, n: nat)
+    requires mf.Valid()
+    requires rf.Valid()
+  {
+    && (|mf.inputs| == rf.input_width * n)
+    && (|mf.outputs| == rf.output_width * n)
+    && (|mf.state| == rf.state_width * n)
+    && (forall si: SI :: SIValid(si, mf.inputs, mf.state) ==>
+      reveal MapFunction.Valid();
+      var so := mf.sf(si);
+      so == ManyParallelSF(rf, n, si))
+  }
+
+  lemma MaintainsMFIsParallelCopies(mf_old: MapFunction, mf_inserted: MapFunction, rf: RFunction, n: nat)
+    requires n > 0
+    requires mf_old.Valid()
+    requires mf_inserted.Valid()
+    requires rf.Valid()
+    requires MFIsParallelCopies(mf_old, rf, n-1)
+    requires rf.MFConsistent(mf_inserted)
+    requires mf_old.NPs() !! mf_inserted.NPs()
+    requires Seq.ToSet(mf_old.state) !! Seq.ToSet(mf_inserted.state)
+    ensures
+      var combiner := ParallelCombiner(mf_old, mf_inserted);
+      var mf_combined := combiner.mf();
+      MFIsParallelCopies(mf_combined, rf, n)      
+  {
+    reveal RFunction.MFConsistent();
+    reveal MFIsParallelCopies();
+    var combiner := ParallelCombiner(mf_old, mf_inserted);
+    var mf := combiner.mf();
+    assert (|mf.inputs| == rf.input_width * n);
+    assert (|mf.outputs| == rf.output_width * n);
+    assert (|mf.state| == rf.state_width * n);
+    forall si: SI | SIValid(si, mf.inputs, mf.state)
+      ensures mf.sf(si) == ManyParallelSF(rf, n, si)
+    {
+      reveal MapFunction.Valid();
+    }
+  }
+
+  lemma MFIsParallelCopiesForSingle(c: Circuit, ei: EntityInserter)
+    requires CircuitValid(c)
+    requires ei.Valid()
+    ensures
+      reveal EntityInserter.Valid();
+      MFIsParallelCopies(ei.fn(c).1.mf, ei.rf, 1)
+  {
+    reveal EntityInserter.Valid();
+    reveal RFunction.Valid();
+    reveal RFunction.MFConsistent();
+    reveal MFIsParallelCopies();
+    var mf := ei.fn(c).1.mf;
+    var rf := ei.rf;
+    forall si: SI | SIValid(si, mf.inputs, mf.state)
+      ensures mf.sf(si) == ManyParallelSF(rf, 1, si)
+    {
+      reveal MapFunction.Valid();
+      var so := mf.sf(si);
+      var chunked_inputs := ChunkSeq(si.inputs, 1, rf.input_width);
+      ChunkSeqSingle(si.inputs);
+      assert chunked_inputs == [si.inputs];
+      var chunked_state := ChunkSeq(si.state, 1, rf.state_width);
+      ChunkSeqSingle(si.state);
+      assert chunked_state == [si.state];
+      var many_si := seq(1, (index: nat) requires index < 1 => SI(chunked_inputs[index], chunked_state[index]));
+      assert many_si == [si];
+      var many_so := seq(1, (index: nat) requires index < 1 => rf.sf(many_si[index]));
+      assert many_so == [so] by  {
+        calc {
+          many_so;
+          seq(1, (index: nat) requires index < 1 => rf.sf(many_si[index]));
+          [rf.sf(many_si[0])];
+          [rf.sf(si)];
+          [mf.sf(si)];
+          [so];
+        }
+      }
+      var chunked_outputs := seq(1, (index: nat) requires index < 1 => many_so[index].outputs);
+      assert chunked_outputs == [so.outputs];
+      var chunked_new_state := seq(1, (index: nat) requires index < 1 => many_so[index].state);
+      assert chunked_new_state == [so.state];
+      var so_outputs := UnchunkSeq(chunked_outputs, 1, rf.output_width);
+      assert so_outputs == so.outputs;
+      var so_state := UnchunkSeq(chunked_new_state, 1, rf.state_width);
+      assert so_state == so.state;
+      var so_other := SO(so_outputs, so_state);
+      assert so_other == so;
+      assert so_other == ManyParallelSF(rf, 1, si);
+    }
+
+  }
+
+  opaque function InsertInParallel(c: Circuit, ei: EntityInserter, n: nat): (r: (Circuit, Entity))
+    requires CircuitValid(c)
+    requires ei.Valid()
+    ensures SimpleInsertion(c, r.0, r.1)
+    ensures
+      reveal EntityInserter.Valid();
+      MFIsParallelCopies(r.1.mf, ei.rf, n)
+  {
+    reveal EntityInserter.Valid();
+    reveal MFIsParallelCopies();
+    if n == 0 then
+      var r := (c, NullEntity);
+      NullEntityValid(c);
+      assert EntityValid(r.0, r.1);
+      assert CircuitUnconnected(c, r.0) by {
+        reveal CircuitUnconnected();
+      }
+      assert CircuitConserved(c, r.0) by {
+        reveal CircuitConserved();
+      }
+      assert IsIsland(r.0, r.1.sc) by {
+        reveal IsIsland();
+      }
+      assert MFIsParallelCopies(r.1.mf, ei.rf, n);
+      r
+    else if n == 1 then
+      var r := ei.fn(c);
+      assert EntityValid(r.0, r.1);
+      assert CircuitUnconnected(c, r.0);
+      assert CircuitConserved(c, r.0);
+      assert IsIsland(r.0, r.1.sc);
+      MFIsParallelCopiesForSingle(c, ei);
+      r
+    else
+      var ib1 := IslandBundleFromCircuit(c);
+
+      var (c_intermed, e_intermed) := InsertInParallel(c, ei, n-1);
+      var (ib2, ref_intermed) := AddEntity(ib1, c_intermed, e_intermed);
+
+      var (new_c, e_inserted) := ei.fn(c_intermed);
+      var (ib3, ref_inserted) := AddEntity(ib2, new_c, e_inserted);
+
+      assert CombineParallelEntitiesRequirements(ib3.c, e_intermed, e_inserted) by {
+        reveal IslandBundleValid();
+      }
+      var (ib4, ref_combined) := IBCombineParallelEntities(ib3, ref_intermed, ref_inserted);
+      var e_combined := ib4.es[ref_combined].value;
+      assert CircuitValid(ib4.c) by {
+        reveal IslandBundleValid();
+      }
+      assert EntityValid(ib4.c, e_combined) by {
+        reveal IslandBundleValid();
+      }
+      assert CircuitUnconnected(c, ib4.c) by {
+        reveal IslandBundleValid();
+      }
+      assert CircuitConserved(c, ib4.c) by {
+        reveal IslandBundleValid();
+      }
+      assert ib4.c.NodeKind.Keys == c.NodeKind.Keys + e_combined.sc by {reveal IslandBundleValid();}
+      assert c.NodeKind.Keys !! e_combined.sc by {reveal IslandBundleValid();}
+      assert IsIsland(ib4.c, e_combined.sc) by {reveal IslandBundleValid();}
+      MaintainsMFIsParallelCopies(e_intermed.mf, e_inserted.mf, ei.rf, n);
+      var r := (ib4.c, e_combined);
+      assert MFIsParallelCopies(r.1.mf, ei.rf, n);
+      assert EntityValid(r.0, r.1);
+      r
+  }
+}
